\section{Yoneda}

\begin{remark}
  The presheaf category $\Set^{\C^\op}$ of $\C$ will be written as $\hat{\C}$.
\end{remark}

\begin{definition}[Yoneda Embedding\index{Yoneda
  Embedding}]\label{def:yoneda_embedding}

  For a locally small category $\C$, the Yoneda embedding $\yo_\C:\C \to
  \hat{\C}$ is defined as maps
  of~\parencite[p.~90]{leinster:basic_category_theory}:

  \begin{itemize}
    \item Objects:
      \[\big(\forall D\in \C_0\big)
        \big(\yo_\C(D) = \C(\hole, D) \big)\]
    \item Morphisms:
      \[\big(\forall h\in \C_1\big)
        \big(\yo_\C(h) = \C(\hole, h) \big)\]
  \end{itemize}
\end{definition}

\begin{remark}
  Note that in line with Remark \ref{rmk:op_hom_functor}, Definition
  \ref{def:yoneda_embedding} can be equaly stated as $\yo_{\C^\op}: \C^\op \to\Set^\C$ as maps of:
  \begin{itemize}
    \item Objects:
      \[\big(\forall C\in \C_0\big)
        \big(\yo_{\C^\op}(c) = \C(C, \hole)\big)\]
    \item Morphisms:
      \[\big(\forall g\in \C_1\big)
        \big(\yo_{\C^\op}(g) = \C(g, \hole)\big)\]
  \end{itemize}
\end{remark}

\begin{theorem}[Yoneda Lemma\index{Yoneda Lemma}\label{thm:yoneda_lemma}]
  For a presheaf $F: \D^\op \to \Set$ on $\D$ and an object $D\in \D_0$, there
  exists a natural isomorphism:
  \[\Set^{(\D^\op)}(\yo_\D(D), F) \cong F(D)\]

  \begin{proof}
    Consider the functions:
    \[
      \begin{gathered}
        \begin{aligned}
          \phi_{\< D, F\>}: \hat{\D}(\yo_\D(D), F) &\to F(D)\\
          \alpha &\mapsto \alpha_D(\id_D)
        \end{aligned}\quad
        \begin{aligned}
          \psi_{\<D, F\>}: F(D) &\to \hat{\D}(\yo_\D(D), F)\\
          X &\mapsto \psi_{\<D, F\>}(X)
        \end{aligned}
      \end{gathered}
    \]

    Such that for $f:C\to D$:
    \[(\psi_{\<D, F\>}(X))_{C}(f) = (F(f))(X)\]

    To prove naturality of $\psi_{\<D, F\>}(X)$, consider a morphism $g:C'\to
    C$:
    % https://q.uiver.app/#q=WzAsNCxbMCwwLCJcXEQoQyxEKSJdLFsxLDAsIkYoQykiXSxbMCwxLCJcXEQoQycsRCkiXSxbMSwxLCJGKEMnKSJdLFswLDEsIihcXHBzaV97XFxsYW5nXFxELCBGXFxyYW5nfShYKSlfQyJdLFsyLDMsIihcXHBzaV97XFxsYW5nIEQsRlxccmFuZ30oWCkpX3tDJ30iLDJdLFswLDIsIlxcRChnLEQpIiwyXSxbMSwzLCJGKGcpIl1d&macro_url=https%3A%2F%2Fraw.githubusercontent.com%2Faortega0703%2Fnotes-category-theory%2Fmain%2Fsrc%2Fmacros.tex
    \[\begin{tikzcd}[ampersand replacement=\&]
      {\D(C,D)} \& {F(C)} \\
      {\D(C',D)} \& {F(C')}
      \arrow["{(\psi_{\langle\D, F\rangle}(X))_C}", from=1-1, to=1-2]
      \arrow["{(\psi_{\langle D,F\rangle}(X))_{C'}}"', from=2-1, to=2-2]
      \arrow["{\D(g,D)}"', from=1-1, to=2-1]
      \arrow["{F(g)}", from=1-2, to=2-2]
    \end{tikzcd}
    \qquad
    \begin{aligned}
        &(F(g)\circ (\psi_{\<d, F\>}(X))_C)(f)\\
        =& F(g)(F(f)(X))\\
        =& F(f\circ g)(X)\\
        =& \psi_{\<D, F\>}(X)_{C'}(f\circ g)
      \end{aligned}
    \]
    Then, consider composition in both ways:
    \[
      \begin{aligned}
        &(\phi \circ \psi)_{\<D, F\>}(X)\\
        =& (\psi_{\<D, F\>}(X))_{D}(\id_D)\\
        =& F(\id_D)(X)\\
        =& \id_{F(D)}(X)\\
        =& X
      \end{aligned}
      \qquad
      \begin{aligned}
        &\big((\psi \circ \phi)_{\<D, F\>}(\alpha)\big)_C(f)\\
        =& \psi_{\<D, F\>} (\alpha_D(\id_D))_C(f)\\
        =& F(f)(\alpha_D(\id_D))\\
        =& \alpha_C(\D(f, D)(\id_D))\\
        =& \alpha_C(f)
      \end{aligned}
    \]
    This proves that $\phi_{\<D, F\>}$ and $\psi_{\<D, F\>}$ form an
    isomorphism. By Theorem \ref{thm:binaturality} to prove that such
    isomorphism is natural on both $D$ and $F$ it suffices to show that it is so
    on each separately. Let $f: D' \to D$ and $\beta: F \to G$, then:
    \[
      \begin{gathered}
        % https://q.uiver.app/#q=WzAsNCxbMCwwLCJcXGhhdHtcXER9KFxceW9fXFxEKEQpLCBGKSJdLFsxLDAsIkYoRCkiXSxbMCwxLCJcXGhhdHtcXER9KFxceW9fXFxEKEQpLCBHKSJdLFsxLDEsIkcoRCkiXSxbMCwxLCJcXHBoaV97XFxsYW5nIEQsIEZcXHJhbmd9Il0sWzAsMiwiXFxoYXR7XFxEfShcXHlvX1xcRChEKSwgXFxiZXRhKSIsMl0sWzIsMywiXFxwaGlfe1xcbGFuZyBELCBGXFxyYW5nfSIsMl0sWzEsMywiXFxiZXRhX0QiXV0=&macro_url=https%3A%2F%2Fgist.githubusercontent.com%2Faortega0703%2Fa1fd97cb097b8142e63a6fbf0cdb0f76%2Fraw%2Fb46a955b6b1f06908105b870088e59a10049fc60%2Fmacros.tex
        \begin{tikzcd}[ampersand replacement=\&]
          {\hat{\D}(\yo_\D(D), F)} \& {F(D)} \\
          {\hat{\D}(\yo_\D(D), G)} \& {G(D)}
          \arrow["{\phi_{\langle D, F\rangle}}", from=1-1, to=1-2]
          \arrow["{\hat{\D}(\yo_\D(D), \beta)}"', from=1-1, to=2-1]
          \arrow["{\phi_{\langle D, F\rangle}}"', from=2-1, to=2-2]
          \arrow["{\beta_D}", from=1-2, to=2-2]
        \end{tikzcd}\\\\\\\\
        % https://q.uiver.app/#q=WzAsNCxbMCwwLCJcXGhhdHtcXER9KFxceW9fXFxEKEQpLCBGKSJdLFsxLDAsIkYoRCkiXSxbMCwxLCJcXGhhdHtcXER9KFxceW9fXFxEKEQnKSwgRikiXSxbMSwxLCJGKEQnKSJdLFswLDEsIlxccGhpX3tcXGxhbmcgRCwgRlxccmFuZ30iXSxbMCwyLCJcXGhhdHtcXER9KFxceW9fXFxEKGYpLCBGKSIsMl0sWzIsMywiXFxwaGlfe1xcbGFuZyBEJywgRlxccmFuZ30iLDJdLFsxLDMsIkYoZikiXV0=&macro_url=https%3A%2F%2Fgist.githubusercontent.com%2Faortega0703%2Fa1fd97cb097b8142e63a6fbf0cdb0f76%2Fraw%2Fb46a955b6b1f06908105b870088e59a10049fc60%2Fmacros.tex
        \begin{tikzcd}[ampersand replacement=\&]
          {\hat{\D}(\yo_\D(D), F)} \& {F(D)} \\
          {\hat{\D}(\yo_\D(D'), F)} \& {F(D')}
          \arrow["{\phi_{\langle D, F\rangle}}", from=1-1, to=1-2]
          \arrow["{\hat{\D}(\yo_\D(f), F)}"', from=1-1, to=2-1]
          \arrow["{\phi_{\langle D', F\rangle}}"', from=2-1, to=2-2]
          \arrow["{F(f)}", from=1-2, to=2-2]
        \end{tikzcd}
      \end{gathered}
      \qquad
      \begin{aligned}
        &(\beta_d \circ \phi_{d, F})(\alpha)\\
        =& \beta_d (\alpha_d (\id_d))\\
        =& (\beta \circ \alpha)_d (\id_d)\\
        =& \phi_{d, F}(\beta \circ \alpha)\\
        =& \phi_{d, F}(\hat{\D}(\yo_\D(d), \beta)(\alpha))\\
        =& (\phi_{d, F} \circ \hat{\D}(\yo_\D(d), \beta)) (\alpha)\\
        %
        \\
        &(F(f)\circ \phi_{d, F}) (\alpha)\\
        =& F(f)(\alpha_d (\id_d))\\
        =& \alpha_{d'}(f)\\
        =& \alpha_{d'}(\yo_\D(f)_{d'}(\id_{d'}))\\
        =& \phi_{d, F}(\alpha \circ \yo_\D(f))\\
        =& \phi_{d, F}(\hat{\D}(\yo_\D(f), F)(\alpha))
      \end{aligned}
    \]
  \end{proof}
  \vspace{-\baselineskip}
\end{theorem}

\begin{remark}
  Note that in line with Remark \ref{rmk:op_hom_functor}, Theorem
  \ref{thm:yoneda_lemma} can be equally stated for a functor $F:\C \to \Set$ and
  an object $C\in\C_0$ as the natural isomorphism:
  \[\Set^{\C}(\yo_{\C^\op}(C), F) \cong F(C)\]
\end{remark}

\begin{theorem}[$\yo$ is Full and Faithful]\label{thm:yoneda_full_faithful} For
  any category $\C$, the Yoneda embedding $\yo_C: \C \to \hat{\C}$ is both full
  and faithful. That is, for every $f: C\to D$ the following is a bijection:
  \[
    \begin{aligned}
      \yo_\C: \C(C, D) &\to \hat{\C}(\yo_\C(C), \yo_\C(D))\\
      f &\mapsto \yo_\C(f)
    \end{aligned}
  \]

  \begin{proof}
    First, consider:
    \[
      \begin{aligned}
        \phi(\yo_\C(f))
        &= (\yo_\C(f))_c(\id_C)\\
        &= \C(C, f) (\id_C)\\
        &= f \circ \id_C\\
        &= f
      \end{aligned}
    \]

    Now, as $\phi(\yo_\C(f)) = f$, then $\yo_\C(f) = \psi(f)$. Finally, by
    Theorem \ref{thm:yoneda_lemma} on $C\in\C_0$ and $\yo_\C(D)$, the following
    is a bijection:
    \[\psi: \C(C,D) \overset{\cong}{\to} \hat{\C}(\yo_\C(C), \yo_\C(D))\]
  \end{proof}
  \vspace{-\baselineskip}
\end{theorem}

\begin{theorem}[Isomorphism Between Yoneda Embeddings]
  For any objects $C, D\in\C_0$:
  \[ C \cong D \iff \yo(C) \cong \yo(D) \]

  \begin{proof}
    It follows immediately from Theorems \ref{thm:full_faithful_isomorphism} and
    \ref{thm:yoneda_full_faithful}.
  \end{proof}
\end{theorem}