\subsection{Classification of Functors}

\begin{definition}[Faithful Functor\index{Faithful Functor}]
  A functor $F:\C\to \D$ is faithful when for every morphism $(f: c\to c') \in
  \C_1$, the following function is
  injective~\parencite[p.~25]{leinster:basic_category_theory}:
    \[
      \begin{aligned}
        F: \C(c, c') &\to \D(F(c), F(c'))\\
        f &\mapsto F(f)
      \end{aligned}
    \]
\end{definition}

\begin{definition}[Full Functor\index{Full Functor}]
  A functor $F:\C\to \D$ is full when for every morphism $(f: c\to c') \in
  \C_1$, the following function is
  surjective~\parencite[p.~25]{leinster:basic_category_theory}:
  \[
    \begin{aligned}
      F: \C(c, c') &\to \D(F(c), F(c'))\\
      f &\mapsto F(f)
    \end{aligned}
  \]
\end{definition}

\begin{definition}[Endofunctor\index{Endofunctor}]
  A functor whose domain equals its codomain is an
  endofunctor~\parencite[p.~30]{adamek_herrlich_strecker:joy_cats}.
\end{definition}

\begin{definition}[Bifunctor\index{Bifunctor}]
  A functor $F:\A\times \B \to \C$ (one with $2$ parameters) is said to be a
  bifunctor~\parencite[p.~37]{lane:working_mathematician}.
\end{definition}

\begin{definition}[Presheaf\index{Presheaf}]
  A functor $\C^\op \to \Set$ is a presheaf on
  $\C$~\parencite[p.~24]{leinster:basic_category_theory}.
\end{definition}

\begin{theorem}[Fully Faithful Isomorphism]\label{thm:full_faithful_isomorphism}

  For any full and faithful functor $F:\C\to \D$ it follows that $c \cong c'
  \iff F(c) \cong F(c')$ for objects $c, c'\in \C_0$.

  \begin{proof}
    The $(\implies)$ holds via Theorem \ref{thm:isomorphism_functor}. For the
    $(\impliedby)$ part, consider the isomorphism $Ff: F(c) \overset{\cong}{\to}
    F(c')$. As $F$ is fully faithful, morphisms $c\to c'$ are in bijection
    with morphisms $F(c)\to F(c')$, therefore there exists unique arrows $f:c\to c'$ $g:c'\to c$ such that $F(f) = Ff$ and $F(g) = Ff^{-1}$, then:
    \[
      \begin{aligned}
        &F(\id_c)\\
        =& \id_{F(c)}\\
        =& Ff^{-1} \circ Ff\\
        =& F(g) \circ F(f)\\
        =& F(g\circ f)
      \end{aligned}
      \qquad
      \begin{aligned}
        &F(\id_{c'})\\
        =& \id_{F(c')}\\
        =& Ff \circ Ff^{-1}\\
        =& F(f) \circ F(g)\\
        =& F(f\circ g)
      \end{aligned}
    \]

    As $F$ is faithful and $F(\id_c) = F(g\circ f)$, then $g\circ f = \id_c$.
    Similarly, $f\circ g = \id_{c'}$.
  \end{proof}
\end{theorem}