\section{Natural Transformations}

\subsection{Definition}
A natural transformation $\alpha : F \Rightarrow G$ from a functor $F:C \to D$
to a functor $G: C \to D$ consists of: \parencite{fong_spivak:7sketches}

\begin{itemize}
  \item $c$-Components:\\
    $(\alpha_c : F(c) \to G(c)) \in D,\ (\forall c\in \ob_C)$\\
    If every $c$-component is an isomorphism the natural transformation is then
    called a natural isomorphism.
  \item Naturality Condition:\\
    The following diagram must commute\footnote{Parallel morphisms i.e. those
    with the same source and target, are equal} for all $c,c'\in C$ and $(f:c\to
    c')\in C$:
    % https://q.uiver.app/?q=WzAsNCxbMCwwLCJGKGMpIl0sWzEsMCwiRihjJykiXSxbMCwxLCJHKGMpIl0sWzEsMSwiRyhjJykiXSxbMCwyLCJcXGFscGhhX2MiXSxbMSwzLCJcXGFscGhhX3tjJ30iXSxbMCwxLCJGKGYpIl0sWzIsMywiRyhmKSIsMl1d
    \[\begin{tikzcd}
      {F(c)} & {F(c')} \\
      {G(c)} & {G(c')}
      \arrow["{\alpha_c}", from=1-1, to=2-1]
      \arrow["{\alpha_{c'}}", from=1-2, to=2-2]
      \arrow["{F(f)}", from=1-1, to=1-2]
      \arrow["{G(f)}"', from=2-1, to=2-2]
    \end{tikzcd}\]
    e.g.
    % https://q.uiver.app/?q=WzAsMTAsWzIsMSwiMSJdLFszLDEsIkYoYSkiXSxbNCwxLCJGKGIpIl0sWzMsMiwiRyhhKSJdLFs0LDIsIkcoYikiXSxbNSwxLCI2Il0sWzAsMSwiYSJdLFsxLDEsImIiXSxbMSwwLCJDIl0sWzIsMCwiRCJdLFswLDEsImciXSxbMCwzLCJoIiwyXSxbMSwzLCJcXGFscGhhX2EiXSxbMiw0LCJcXGFscGhhX2IiLDJdLFsxLDIsIkYoZikiXSxbMyw0LCJHKGYpIiwyXSxbMiw1LCJpIl0sWzQsNSwiaiIsMl0sWzYsNywiZiJdLFs2LDEsIiIsMCx7ImN1cnZlIjotMywiY29sb3VyIjpbMjQwLDYwLDYwXSwic3R5bGUiOnsiYm9keSI6eyJuYW1lIjoiZG90dGVkIn19fV0sWzcsMiwiIiwyLHsiY3VydmUiOi0zLCJjb2xvdXIiOlsyNDAsNjAsNjBdLCJzdHlsZSI6eyJib2R5Ijp7Im5hbWUiOiJkb3R0ZWQifX19XSxbNiwzLCIiLDIseyJjb2xvdXIiOlswLDYwLDYwXSwic3R5bGUiOnsiYm9keSI6eyJuYW1lIjoiZG90dGVkIn19fV0sWzcsNCwiIiwyLHsiY29sb3VyIjpbMCw2MCw2MF0sInN0eWxlIjp7ImJvZHkiOnsibmFtZSI6ImRvdHRlZCJ9fX1dLFs4LDksIkYiLDEseyJjdXJ2ZSI6LTMsImNvbG91ciI6WzI0MCw2MCw2MF19XSxbOCw5LCJHIiwxLHsiY3VydmUiOjMsImNvbG91ciI6WzAsNjAsNjBdfV1d
    \[\begin{tikzcd}
      & C & D \\
      a & b & 1 & {F(a)} & {F(b)} & 6 \\
      &&& {G(a)} & {G(b)}
      \arrow["g", from=2-3, to=2-4]
      \arrow["h"', from=2-3, to=3-4]
      \arrow["{\alpha_a}", from=2-4, to=3-4]
      \arrow["{\alpha_b}"', from=2-5, to=3-5]
      \arrow["{F(f)}", from=2-4, to=2-5]
      \arrow["{G(f)}"', from=3-4, to=3-5]
      \arrow["i", from=2-5, to=2-6]
      \arrow["j"', from=3-5, to=2-6]
      \arrow["f", from=2-1, to=2-2]
      \arrow[draw={rgb,255:red,92;green,92;blue,214}, curve={height=-18pt}, dotted, from=2-1, to=2-4]
      \arrow[draw={rgb,255:red,92;green,92;blue,214}, curve={height=-18pt}, dotted, from=2-2, to=2-5]
      \arrow[draw={rgb,255:red,214;green,92;blue,92}, dotted, from=2-1, to=3-4]
      \arrow[draw={rgb,255:red,214;green,92;blue,92}, dotted, from=2-2, to=3-5]
      \arrow["F"{description}, draw={rgb,255:red,92;green,92;blue,214}, curve={height=-18pt}, from=1-2, to=1-3]
      \arrow["G"{description}, draw={rgb,255:red,214;green,92;blue,92}, curve={height=18pt}, from=1-2, to=1-3]
    \end{tikzcd}\]
\end{itemize}

\subsection{Identity}
For any categories $C,D$ with a functor $F:C\to D$, there exists a natural
transformation $\id_F: F\Rightarrow F$ which consists of:
\parencite{leinster:basic_category_theory}
\begin{itemize}
  \item $c$-Components:\\
    $(\id_F)_c: F(c) \to F(c) = \id_{F(c)},\ (\forall c\in C)$
  \item Naturality Condition:
    % https://q.uiver.app/?q=WzAsNCxbMCwwLCJGKGMpIl0sWzEsMCwiRihjJykiXSxbMCwxLCJGKGMpIl0sWzEsMSwiRihjJykiXSxbMCwxLCJGKGYpIl0sWzAsMiwiXFxtYXRocm17aWR9X3tGKGMpfSIsMl0sWzIsMywiRihmKSIsMl0sWzEsMywiXFxtYXRocm17aWR9X3tGKGMpfSJdXQ==
    \[\begin{tikzcd}
      {F(c)} & {F(c')} \\
      {F(c)} & {F(c')}
      \arrow["{F(f)}", from=1-1, to=1-2]
      \arrow["{\id_{F(c)}}"', from=1-1, to=2-1]
      \arrow["{F(f)}"', from=2-1, to=2-2]
      \arrow["{\id_{F(c)}}", from=1-2, to=2-2]
    \end{tikzcd}\]
    Which commutes for all $c,c'\in C$ and $(f:c\to c')\in C$ by using
    unitality of $D$.
\end{itemize}

\subsection{Vertical Composition}
For categories $C,D$ with functors $F,G,H:C\to D$ and natural transformations
$\alpha:F\to G,\ \beta:G\to H$, the vertical composition $\beta\circ \alpha:F\to
H$ consists of: \parencite{leinster:basic_category_theory}

\begin{itemize}
  \item $c$-Components:\\
    $(\beta\circ\alpha)_c: F(c) \to H(c) = \beta_c \circ \alpha_c,\ (\forall
    c\in C)$
  \item Naturality Condition:
    % https://q.uiver.app/?q=WzAsNixbMCwwLCJGKGMpIl0sWzEsMCwiRihjJykiXSxbMCwxLCJHKGMpIl0sWzAsMiwiSChjKSJdLFsxLDEsIkcoYycpIl0sWzEsMiwiSChjJykiXSxbMCwxLCJGKGYpIiwwLHsiY29sb3VyIjpbMjQwLDYwLDYwXX1dLFsyLDQsIkcoZikiXSxbMyw1LCJIKGYpIiwyLHsiY29sb3VyIjpbMjQwLDYwLDYwXX1dLFswLDIsIlxcYWxwaGFfYyIsMV0sWzIsMywiXFxiZXRhX2MiLDFdLFsxLDQsIlxcYWxwaGFfe2MnfSIsMV0sWzQsNSwiXFxiZXRhX3tjJ30iLDFdLFswLDMsIihcXGJldGFcXGNpcmNcXGFscGhhKV9jIiwyLHsiY3VydmUiOjQsImNvbG91ciI6WzI0MCw2MCw2MF19XSxbMSw1LCIoXFxiZXRhXFxjaXJjXFxhbHBoYSlfe2MnfSIsMCx7ImN1cnZlIjotNCwiY29sb3VyIjpbMjQwLDYwLDYwXX1dXQ==
    \[\begin{tikzcd}
      {F(c)} & {F(c')} \\
      {G(c)} & {G(c')} \\
      {H(c)} & {H(c')}
      \arrow["{F(f)}", draw={rgb,255:red,92;green,92;blue,214}, from=1-1, to=1-2]
      \arrow["{G(f)}", from=2-1, to=2-2]
      \arrow["{H(f)}"', draw={rgb,255:red,92;green,92;blue,214}, from=3-1, to=3-2]
      \arrow["{\alpha_c}"{description}, from=1-1, to=2-1]
      \arrow["{\beta_c}"{description}, from=2-1, to=3-1]
      \arrow["{\alpha_{c'}}"{description}, from=1-2, to=2-2]
      \arrow["{\beta_{c'}}"{description}, from=2-2, to=3-2]
      \arrow["{(\beta\circ\alpha)_c}"', draw={rgb,255:red,92;green,92;blue,214}, curve={height=24pt}, from=1-1, to=3-1]
      \arrow["{(\beta\circ\alpha)_{c'}}", draw={rgb,255:red,92;green,92;blue,214}, curve={height=-24pt}, from=1-2, to=3-2]
    \end{tikzcd}\]

    The naturality conditions of $\alpha$ and $\beta$ imply the naturality
    condition of $\beta \circ \alpha$ (in blue):
    \[
      \begin{aligned}
        \beta_{c'}\circ\alpha_{c'}\circ F(f)
        &= \beta_{c'}\circ G(f) \circ\alpha_c
          ,\quad\text{(naturality condition of $\alpha$)}\\
        &= H(f)\circ \beta_c \circ \alpha_c
          ,\quad\text{(naturality condition of $\beta$)}
      \end{aligned}
    \]
\end{itemize}

\subsubsection*{Unitality of Vertical Composition}
For categories $C,D$, functors $F,G:C\to D$, a natural tranformation $\alpha:
F\Rightarrow G$ and $c\in C$, consider its vertical composition with the
identity natural transformations:

\[
  \begin{aligned}
    (\alpha \circ \id_F)_C
    &= \alpha_c \circ (\id_F)_c\\
    &= \alpha_c \circ \id_{F(c)}\\
    &= \alpha_c
  \end{aligned}
  \quad
  \begin{aligned}
    (\id_G \circ \alpha)_c
    &= (\id_G)_c \circ \alpha_c\\
    &= \id_{G(c)} \circ \alpha_c\\
    &= \alpha_c
  \end{aligned}
\]

Therefore $\alpha \circ \id_F = \id_G \circ \alpha = \alpha$.

\subsubsection*{Associativity of Vertical Composition}
For categories $C,D$, functors $F,G,H,I:C\to D$, natural tranformations $\alpha:
F\Rightarrow G, \beta: G\Rightarrow H, \gamma:H\Rightarrow I$ and $c\in C$,
consider their vertical composition:

\[
  \begin{aligned}
    ((\gamma \circ \beta) \circ \alpha)_c
    &= (\gamma \circ \beta)_c \circ \alpha_c\\
    &= (\gamma_c \circ \beta_c) \circ \alpha_c\\
    &= \gamma_c \circ (\beta_c \circ \alpha_c)
      ,\quad\text{(associativity of morphisms)}\\
    &= \gamma_c \circ (\beta \circ \alpha)_c\\
    &= (\gamma \circ (\beta \circ \alpha))_c\\
  \end{aligned}
\]

Therefore $(\gamma \circ \beta) \circ \alpha = \gamma \circ (\beta \circ
\alpha)$

\subsection{Horizontal Composition}
For categories $A,B,C$, functors $F,F':A\to B$ and $G,G':B\to C$, and natural
transformations $\alpha: F\Rightarrow F'$ and $\beta:G\to G'$, the horizontal
composition $\beta * \alpha: (G\circ F) \to (G' \circ F')$ consists of:
\parencite{leinster:basic_category_theory}

\begin{itemize}
  \item $c$-Components:\\
    $(\beta * \alpha)_c : (G\circ F) \to (G' \circ F') =\beta_{F'(c)} \circ
    G(\alpha_c)\in C$\\
    \phantom{$(\beta * \alpha)_c : (G\circ F) \to (G' \circ F')$}
    $= G'(\alpha_c) \circ \beta_{F(c)}\in C$\\
    This definition is motivated by the following diagram, where the equality of
    both definitions is given by the naturality condition of $\beta$.

    % https://q.uiver.app/?q=WzAsMTAsWzAsMCwiQSJdLFswLDIsImMiXSxbMSwwLCJCIl0sWzIsMCwiQyJdLFsxLDEsIkYoYykiXSxbMSwzLCJGJyhjKSJdLFsyLDIsIihHXFxjaXJjIEYpKGMpIl0sWzMsMSwiKEcnXFxjaXJjIEYpKGMpIl0sWzIsNCwiKEdcXGNpcmMgRicpKGMpIl0sWzMsMywiKEcnXFxjaXJjIEYnKShjKSJdLFswLDIsIkYiLDAseyJjdXJ2ZSI6LTIsImNvbG91ciI6WzI0MCw2MCw2MF19XSxbMCwyLCJGJyIsMix7ImN1cnZlIjoyLCJjb2xvdXIiOlswLDYwLDYwXX1dLFsyLDMsIkciLDAseyJjdXJ2ZSI6LTIsImNvbG91ciI6WzI0MCw2MCw2MF19XSxbMiwzLCJHJyIsMix7ImN1cnZlIjoyLCJjb2xvdXIiOlswLDYwLDYwXX1dLFsxLDQsIiIsMCx7ImNvbG91ciI6WzI0MCw2MCw2MF0sInN0eWxlIjp7ImJvZHkiOnsibmFtZSI6ImRvdHRlZCJ9fX1dLFsxLDUsIiIsMix7ImNvbG91ciI6WzAsNjAsNjBdLCJzdHlsZSI6eyJib2R5Ijp7Im5hbWUiOiJkb3R0ZWQifX19XSxbNCw1LCJcXGFscGhhX2MiXSxbNCw2LCIiLDAseyJjb2xvdXIiOlsyNDAsNjAsNjBdLCJzdHlsZSI6eyJib2R5Ijp7Im5hbWUiOiJkb3R0ZWQifX19XSxbNCw3LCIiLDAseyJjb2xvdXIiOlswLDYwLDYwXSwic3R5bGUiOnsiYm9keSI6eyJuYW1lIjoiZG90dGVkIn19fV0sWzUsOCwiIiwwLHsiY29sb3VyIjpbMjQwLDYwLDYwXSwic3R5bGUiOnsiYm9keSI6eyJuYW1lIjoiZG90dGVkIn19fV0sWzUsOSwiIiwwLHsiY29sb3VyIjpbMCw2MCw2MF0sInN0eWxlIjp7ImJvZHkiOnsibmFtZSI6ImRvdHRlZCJ9fX1dLFs2LDcsIlxcYmV0YV97RihjKX0iXSxbOCw5LCJcXGJldGFfe0YnKGMpfSIsMl0sWzcsOSwiRycoXFxhbHBoYV9jKSJdLFs2LDgsIkcoXFxhbHBoYV9jKSJdLFs2LDksIlxcYmV0YSpcXGFscGhhIl0sWzEyLDEzLCJcXGJldGEiLDAseyJzaG9ydGVuIjp7InNvdXJjZSI6MjAsInRhcmdldCI6MjB9fV0sWzEwLDExLCJcXGFscGhhIiwwLHsic2hvcnRlbiI6eyJzb3VyY2UiOjIwLCJ0YXJnZXQiOjIwfX1dXQ==
    \[\begin{tikzcd}
      A & B & C \\
      & {F(c)} && {(G'\circ F)(c)} \\
      c && {(G\circ F)(c)} \\
      & {F'(c)} && {(G'\circ F')(c)} \\
      && {(G\circ F')(c)}
      \arrow[""{name=0, anchor=center, inner sep=0}, "F", draw={rgb,255:red,92;green,92;blue,214}, curve={height=-12pt}, from=1-1, to=1-2]
      \arrow[""{name=1, anchor=center, inner sep=0}, "{F'}"', draw={rgb,255:red,214;green,92;blue,92}, curve={height=12pt}, from=1-1, to=1-2]
      \arrow[""{name=2, anchor=center, inner sep=0}, "G", draw={rgb,255:red,92;green,92;blue,214}, curve={height=-12pt}, from=1-2, to=1-3]
      \arrow[""{name=3, anchor=center, inner sep=0}, "{G'}"', draw={rgb,255:red,214;green,92;blue,92}, curve={height=12pt}, from=1-2, to=1-3]
      \arrow[color={rgb,255:red,92;green,92;blue,214}, dotted, from=3-1, to=2-2]
      \arrow[color={rgb,255:red,214;green,92;blue,92}, dotted, from=3-1, to=4-2]
      \arrow["{\alpha_c}", from=2-2, to=4-2]
      \arrow[color={rgb,255:red,92;green,92;blue,214}, dotted, from=2-2, to=3-3]
      \arrow[color={rgb,255:red,214;green,92;blue,92}, dotted, from=2-2, to=2-4]
      \arrow[color={rgb,255:red,92;green,92;blue,214}, dotted, from=4-2, to=5-3]
      \arrow[color={rgb,255:red,214;green,92;blue,92}, dotted, from=4-2, to=4-4]
      \arrow["{\beta_{F(c)}}", from=3-3, to=2-4]
      \arrow["{\beta_{F'(c)}}"', from=5-3, to=4-4]
      \arrow["{G'(\alpha_c)}", from=2-4, to=4-4]
      \arrow["{G(\alpha_c)}", from=3-3, to=5-3]
      \arrow["{\beta*\alpha}", from=3-3, to=4-4]
      \arrow["\beta", shorten <=3pt, shorten >=3pt, Rightarrow, from=2, to=3]
      \arrow["\alpha", shorten <=3pt, shorten >=3pt, Rightarrow, from=0, to=1]
    \end{tikzcd}\]
  \item Naturality Condition:
    % https://q.uiver.app/?q=WzAsOCxbMSwwLCIoR1xcY2lyYyBGKShjKSJdLFszLDAsIihHJ1xcY2lyYyBGKShjKSJdLFsxLDIsIihHXFxjaXJjIEYnKShjKSJdLFszLDIsIihHJ1xcY2lyYyBGJykoYykiXSxbMiw0LCIoRydcXGNpcmMgRikoYycpIl0sWzAsNCwiKEdcXGNpcmMgRikoYycpIl0sWzAsNiwiKEdcXGNpcmMgRicpKGMnKSJdLFsyLDYsIihHJ1xcY2lyYyBGJykoYycpIl0sWzAsMiwiRyhcXGFscGhhX2MpIiwxXSxbMiwzLCJcXGJldGFfe0YnKGMpfSIsMV0sWzAsMSwiXFxiZXRhX3tGKGMpfSIsMV0sWzEsMywiRycoXFxhbHBoYV9jKSIsMV0sWzAsNSwiKEdcXGNpcmMgRikoZikiLDEseyJsYWJlbF9wb3NpdGlvbiI6NjAsImNvbG91ciI6WzI0MCw2MCw2MF19XSxbMiw2LCIoR1xcY2lyYyBGJykoZikiLDEseyJsYWJlbF9wb3NpdGlvbiI6MzB9XSxbMSw0LCIoRydcXGNpcmMgRikoZikiLDEseyJsYWJlbF9wb3NpdGlvbiI6NzB9XSxbMyw3LCIoRydcXGNpcmMgRicpKGYpIiwxLHsibGFiZWxfcG9zaXRpb24iOjQwLCJjb2xvdXIiOlsyNDAsNjAsNjBdfV0sWzUsNCwiXFxiZXRhX3tGKGMnKX0iLDFdLFs0LDcsIkcnKFxcYWxwaGFfe2MnfSkiLDFdLFs1LDYsIkcoXFxhbHBoYV97Yyd9KSIsMV0sWzYsNywiXFxiZXRhX3tGJyhjKX0iLDFdLFswLDMsIihcXGJldGEgKlxcYWxwaGEpX2MiLDEseyJjb2xvdXIiOlsyNDAsNjAsNjBdLCJzdHlsZSI6eyJib2R5Ijp7Im5hbWUiOiJkb3R0ZWQifX19XSxbNSw3LCIoXFxiZXRhICpcXGFscGhhKV97Yyd9IiwxLHsiY29sb3VyIjpbMjQwLDYwLDYwXSwic3R5bGUiOnsiYm9keSI6eyJuYW1lIjoiZG90dGVkIn19fV1d
    \[\begin{tikzcd}
      & {(G\circ F)(c)} && {(G'\circ F)(c)} \\
      \\
      & {(G\circ F')(c)} && {(G'\circ F')(c)} \\
      \\
      {(G\circ F)(c')} && {(G'\circ F)(c')} \\
      \\
      {(G\circ F')(c')} && {(G'\circ F')(c')}
      \arrow["{G(\alpha_c)}"{description}, from=1-2, to=3-2]
      \arrow["{\beta_{F'(c)}}"{description}, from=3-2, to=3-4]
      \arrow["{\beta_{F(c)}}"{description}, from=1-2, to=1-4]
      \arrow["{G'(\alpha_c)}"{description}, from=1-4, to=3-4]
      \arrow["{(G\circ F)(f)}"{description, pos=0.6}, draw={rgb,255:red,92;green,92;blue,214}, from=1-2, to=5-1]
      \arrow["{(G\circ F')(f)}"{description, pos=0.3}, from=3-2, to=7-1]
      \arrow["{(G'\circ F)(f)}"{description, pos=0.7}, from=1-4, to=5-3]
      \arrow["{(G'\circ F')(f)}"{description, pos=0.4}, draw={rgb,255:red,92;green,92;blue,214}, from=3-4, to=7-3]
      \arrow["{\beta_{F(c')}}"{description}, from=5-1, to=5-3]
      \arrow["{G'(\alpha_{c'})}"{description}, from=5-3, to=7-3]
      \arrow["{G(\alpha_{c'})}"{description}, from=5-1, to=7-1]
      \arrow["{\beta_{F'(c)}}"{description}, from=7-1, to=7-3]
      \arrow["{(\beta *\alpha)_c}"{description}, draw={rgb,255:red,92;green,92;blue,214}, dotted, from=1-2, to=3-4]
      \arrow["{(\beta *\alpha)_{c'}}"{description}, draw={rgb,255:red,92;green,92;blue,214}, dotted, from=5-1, to=7-3]
    \end{tikzcd}\]
    The naturality conditions of $\alpha$ and $\beta$ imply the naturality
    condition of $\beta * \alpha$ (in blue):

    \[
      \begin{aligned}
        (G'\circ F')(f) \circ (\beta * \alpha)_c
        &= (G'\circ F')(f) \circ G'(\alpha_c)\circ\beta_{F(c)}\\
        &= G'(\alpha_{c'}) \circ (G' \circ F)(f) \circ \beta_{F(c)}
          ,\quad\text{(naturality condition of $\alpha$)}\\
        &= G'(\alpha_{c'}) \circ \beta_{F(c')} \circ (G \circ F)(f)
          ,\quad\text{(naturality condition of $\beta$)}\\
        &= (\beta * \alpha)_{c'}\circ (G \circ F)(f)
      \end{aligned}
    \]
\end{itemize}

\subsubsection*{Unitality of Horizontal Composition}
For categories $C,D$, functors $F,G:C\to D$, a natural tranformation $\alpha:
F\Rightarrow G$ and $c\in C$, consider its horizontal composition with the
identity natural transformation of the identity functor:

\[
  \begin{aligned}[t]
    (\alpha * \id_{\id_C})_c
    &= \alpha_{\id_C(c)} \circ F((\id_{\id_C})_c)\\
    &= \alpha_{c} \circ F(\id_{\id_C(c)})\\
    &= \alpha_{c} \circ F(\id_{c})\\
    &= \alpha_{c} \circ \id_{F(c)}\\
    &= \alpha_{c}
  \end{aligned}
  \quad
  \begin{aligned}[t]
    (\id_{\id_D} * \alpha)_c
    &= (\id_{\id_D})_{G(c)} \circ \id_D(\alpha_c)\\
    &= \id_{\id_D(G(c))} \circ \alpha_c\\
    &= \id_{G(c)} \circ \alpha_c\\
    &= \alpha_c
  \end{aligned}
\]

Therefore $\alpha * \id_{\id_C} = \id_{\id_D} * \alpha = \alpha$.

\subsubsection*{Associativity of Horizontal Composition}
For categories $A,B,C,D$, functos $F,F': A\to B$, $G,G':B\to C$, $H,H':C\to D$,
natural transformations $\alpha:F\Rightarrow F'$, $\beta:G\Rightarrow G'$,
$\gamma: H\Rightarrow H'$ and $a\in A$, consider their horizontal composition:
\[
  \begin{aligned}
    ((\gamma * \beta) * \alpha)_a
    &= (\gamma * \beta)_{F'(a)} \circ (H\circ G)(\alpha_a)\\
    &= \left(\gamma_{(G'\circ F')(a)}\circ H(\beta_{F'(a)})\right)
    \circ (H\circ G)(\alpha_a)\\
    &= \gamma_{(G'\circ F')(a)} \circ
    \left(H(\beta_{F'(a)}) \circ (H\circ G)(\alpha_a)\right)
    ,\quad\text{(associativity of $\circ$)}\\
    &= \gamma_{(G'\circ F')(a)}\circ
    H\left((\beta_{F'(a)}) \circ G(\alpha_a)\right)
    ,\quad\text{(preservation of $\circ$ over $H$)}\\
    &= \gamma_{(G'\circ F')(a)} \circ H( (\beta *\alpha)_a)\\
    &= \gamma * (\beta * \alpha)_a
  \end{aligned}
\]