\subsection{Horizontal Composition}

\begin{definition}[Horizontal Composition]\index{Horizontal
  Composition}\label{def:nat_transformation_cmp2}
  For a set-up of categories, functors, and natural transformations:
  % https://q.uiver.app/?q=WzAsMyxbMCwwLCJcXEEiXSxbMiwwLCJcXEIiXSxbNCwwLCJcXEMiXSxbMCwxLCJGIiwxLHsiY3VydmUiOi00fV0sWzAsMSwiRiciLDEseyJjdXJ2ZSI6NH1dLFsxLDIsIkciLDEseyJjdXJ2ZSI6LTR9XSxbMSwyLCJHJyIsMSx7ImN1cnZlIjo0fV0sWzMsNCwiXFxhbHBoYSIsMCx7InNob3J0ZW4iOnsic291cmNlIjoyMCwidGFyZ2V0IjoyMH19XSxbNSw2LCJcXGJldGEiLDAseyJzaG9ydGVuIjp7InNvdXJjZSI6MjAsInRhcmdldCI6MjB9fV1d&macro_url=https%3A%2F%2Fraw.githubusercontent.com%2Faortega0703%2Fnotes-category-theory%2Fmain%2Fsrc%2Fmacros.tex
  \[\begin{tikzcd}[ampersand replacement=\&]
    \A \&\& \B \&\& \C
    \arrow[""{name=0, anchor=center, inner sep=0}, "F"{description}, curve={height=-24pt}, from=1-1, to=1-3]
    \arrow[""{name=1, anchor=center, inner sep=0}, "{F'}"{description}, curve={height=24pt}, from=1-1, to=1-3]
    \arrow[""{name=2, anchor=center, inner sep=0}, "G"{description}, curve={height=-24pt}, from=1-3, to=1-5]
    \arrow[""{name=3, anchor=center, inner sep=0}, "{G'}"{description}, curve={height=24pt}, from=1-3, to=1-5]
    \arrow["\alpha", shorten <=6pt, shorten >=6pt, Rightarrow, from=0, to=1]
    \arrow["\beta", shorten <=6pt, shorten >=6pt, Rightarrow, from=2, to=3]
  \end{tikzcd}\]

  The horizontal composition $\beta * \alpha: (G\circ F) \to (G' \circ F')$
  consists of~\parencite[p.~37]{leinster:basic_category_theory}:
  \begin{itemize}
    \item $C$-Components:
      \[(\forall C\in\C_0)
        \big((\beta * \alpha)_C
        =\beta_{F'(C)} \circ G(\alpha_C)
        = G'(\alpha_C) \circ \beta_{F(C)}\big)
      \]
    \item Naturality Condition:
      % https://q.uiver.app/#q=WzAsNCxbMCwwLCIoR1xcY2lyYyBGKShDKSJdLFswLDIsIihHJ1xcY2lyYyBGJykoQykiXSxbMiwwLCIoR1xcY2lyYyBGKShEKSJdLFsyLDIsIihHJ1xcY2lyYyBGJykoRCkiXSxbMCwyLCIoR1xcY2lyYyBGKShmKSJdLFsxLDMsIihHJ1xcY2lyYyBGJykoZikiLDJdLFswLDEsIihcXGJldGEgKlxcYWxwaGEpX0MiLDFdLFsyLDMsIihcXGJldGEgKlxcYWxwaGEpX3tEfSIsMV1d
      \[\begin{tikzcd}[ampersand replacement=\&]
        {(G\circ F)(C)} \&\& {(G\circ F)(D)} \\
        \\
        {(G'\circ F')(C)} \&\& {(G'\circ F')(D)}
        \arrow["{(G\circ F)(f)}", from=1-1, to=1-3]
        \arrow["{(G'\circ F')(f)}"', from=3-1, to=3-3]
        \arrow["{(\beta *\alpha)_C}"{description}, from=1-1, to=3-1]
        \arrow["{(\beta *\alpha)_{D}}"{description}, from=1-3, to=3-3]
      \end{tikzcd}\]
  \end{itemize}
\end{definition}

\begin{remark}
  The definition of the $C$-components for horizontal composition is motivated
  by the following diagram, where the equality of both definitions is given by
  the naturality condition of $\beta$.

  % https://q.uiver.app/#q=WzAsNyxbMCwwLCJDIl0sWzEsMCwiRihDKSJdLFsxLDIsIkYnKEMpIl0sWzIsMSwiKEdcXGNpcmMgRikoQykiXSxbMywwLCIoRydcXGNpcmMgRikoQykiXSxbMiwzLCIoR1xcY2lyYyBGJykoQykiXSxbMywyLCIoRydcXGNpcmMgRicpKEMpIl0sWzAsMSwiIiwwLHsiY29sb3VyIjpbMjQwLDYwLDYwXSwic3R5bGUiOnsiYm9keSI6eyJuYW1lIjoiZG90dGVkIn19fV0sWzAsMiwiIiwyLHsiY29sb3VyIjpbMCw2MCw2MF0sInN0eWxlIjp7ImJvZHkiOnsibmFtZSI6ImRvdHRlZCJ9fX1dLFsxLDIsIlxcYWxwaGFfQyIsMV0sWzEsMywiIiwwLHsiY29sb3VyIjpbMjQwLDYwLDYwXSwic3R5bGUiOnsiYm9keSI6eyJuYW1lIjoiZG90dGVkIn19fV0sWzEsNCwiIiwwLHsiY29sb3VyIjpbMCw2MCw2MF0sInN0eWxlIjp7ImJvZHkiOnsibmFtZSI6ImRvdHRlZCJ9fX1dLFsyLDUsIiIsMCx7ImNvbG91ciI6WzI0MCw2MCw2MF0sInN0eWxlIjp7ImJvZHkiOnsibmFtZSI6ImRvdHRlZCJ9fX1dLFsyLDYsIiIsMCx7ImNvbG91ciI6WzAsNjAsNjBdLCJzdHlsZSI6eyJib2R5Ijp7Im5hbWUiOiJkb3R0ZWQifX19XSxbMyw0LCJcXGJldGFfe0YoQyl9IiwxXSxbNSw2LCJcXGJldGFfe0YnKEMpfSIsMV0sWzQsNiwiRycoXFxhbHBoYV9DKSIsMV0sWzMsNSwiRyhcXGFscGhhX0MpIiwxXSxbMyw2LCIoXFxiZXRhKlxcYWxwaGEpX0MiLDFdXQ==
  \[\begin{tikzcd}[ampersand replacement=\&]
    C \& {F(C)} \&\& {(G'\circ F)(C)} \\
    \&\& {(G\circ F)(C)} \\
    \& {F'(C)} \&\& {(G'\circ F')(C)} \\
    \&\& {(G\circ F')(C)}
    \arrow[draw={rgb,255:red,92;green,92;blue,214}, dotted, from=1-1, to=1-2]
    \arrow[draw={rgb,255:red,214;green,92;blue,92}, dotted, from=1-1, to=3-2]
    \arrow["{\alpha_C}"{description}, from=1-2, to=3-2]
    \arrow[draw={rgb,255:red,92;green,92;blue,214}, dotted, from=1-2, to=2-3]
    \arrow[draw={rgb,255:red,214;green,92;blue,92}, dotted, from=1-2, to=1-4]
    \arrow[draw={rgb,255:red,92;green,92;blue,214}, dotted, from=3-2, to=4-3]
    \arrow[draw={rgb,255:red,214;green,92;blue,92}, dotted, from=3-2, to=3-4]
    \arrow["{\beta_{F(C)}}"{description}, from=2-3, to=1-4]
    \arrow["{\beta_{F'(C)}}"{description}, from=4-3, to=3-4]
    \arrow["{G'(\alpha_C)}"{description}, from=1-4, to=3-4]
    \arrow["{G(\alpha_C)}"{description}, from=2-3, to=4-3]
    \arrow["{(\beta*\alpha)_C}"{description}, from=2-3, to=3-4]
  \end{tikzcd}\]
\end{remark}

\begin{theorem}
  The naturality condition of horizontal composition holds, therefore it is a
  natural transformation.

  \begin{proof}
    % https://q.uiver.app/?q=WzAsOCxbMSwwLCIoR1xcY2lyYyBGKShjKSJdLFszLDAsIihHJ1xcY2lyYyBGKShjKSJdLFsxLDIsIihHXFxjaXJjIEYnKShjKSJdLFszLDIsIihHJ1xcY2lyYyBGJykoYykiXSxbMiw0LCIoRydcXGNpcmMgRikoYycpIl0sWzAsNCwiKEdcXGNpcmMgRikoYycpIl0sWzAsNiwiKEdcXGNpcmMgRicpKGMnKSJdLFsyLDYsIihHJ1xcY2lyYyBGJykoYycpIl0sWzAsMiwiRyhcXGFscGhhX2MpIiwxXSxbMiwzLCJcXGJldGFfe0YnKGMpfSIsMV0sWzAsMSwiXFxiZXRhX3tGKGMpfSIsMV0sWzEsMywiRycoXFxhbHBoYV9jKSIsMV0sWzAsNSwiKEdcXGNpcmMgRikoZikiLDEseyJsYWJlbF9wb3NpdGlvbiI6NjAsImNvbG91ciI6WzI0MCw2MCw2MF19XSxbMiw2LCIoR1xcY2lyYyBGJykoZikiLDEseyJsYWJlbF9wb3NpdGlvbiI6MzB9XSxbMSw0LCIoRydcXGNpcmMgRikoZikiLDEseyJsYWJlbF9wb3NpdGlvbiI6NzB9XSxbMyw3LCIoRydcXGNpcmMgRicpKGYpIiwxLHsibGFiZWxfcG9zaXRpb24iOjQwLCJjb2xvdXIiOlsyNDAsNjAsNjBdfV0sWzUsNCwiXFxiZXRhX3tGKGMnKX0iLDFdLFs0LDcsIkcnKFxcYWxwaGFfe2MnfSkiLDFdLFs1LDYsIkcoXFxhbHBoYV97Yyd9KSIsMV0sWzYsNywiXFxiZXRhX3tGJyhjKX0iLDFdLFswLDMsIihcXGJldGEgKlxcYWxwaGEpX2MiLDEseyJjb2xvdXIiOlsyNDAsNjAsNjBdfV0sWzUsNywiKFxcYmV0YSAqXFxhbHBoYSlfe2MnfSIsMSx7ImNvbG91ciI6WzI0MCw2MCw2MF19XV0=
    \[\begin{tikzcd}[scale cd=0.8,column sep=tiny,row sep=scriptsize]
      & {(G\circ F)(c)} && {(G'\circ F)(c)} \\
      \\
      & {(G\circ F')(c)} && {(G'\circ F')(c)} \\
      \\
      {(G\circ F)(c')} && {(G'\circ F)(c')} \\
      \\
      {(G\circ F')(c')} && {(G'\circ F')(c')}
      \arrow["{G(\alpha_c)}"{description}, from=1-2, to=3-2]
      \arrow["{\beta_{F'(c)}}"{description}, from=3-2, to=3-4]
      \arrow["{\beta_{F(c)}}"{description}, from=1-2, to=1-4]
      \arrow["{G'(\alpha_c)}"{description}, from=1-4, to=3-4]
      \arrow["{(G\circ F)(f)}"{description, pos=0.6}, draw={rgb,255:red,92;green,92;blue,214}, from=1-2, to=5-1]
      \arrow["{(G\circ F')(f)}"{description, pos=0.3}, from=3-2, to=7-1]
      \arrow["{(G'\circ F)(f)}"{description, pos=0.7}, from=1-4, to=5-3]
      \arrow["{(G'\circ F')(f)}"{description, pos=0.4}, draw={rgb,255:red,92;green,92;blue,214}, from=3-4, to=7-3]
      \arrow["{\beta_{F(c')}}"{description}, from=5-1, to=5-3]
      \arrow["{G'(\alpha_{c'})}"{description}, from=5-3, to=7-3]
      \arrow["{G(\alpha_{c'})}"{description}, from=5-1, to=7-1]
      \arrow["{\beta_{F'(c)}}"{description}, from=7-1, to=7-3]
      \arrow["{(\beta *\alpha)_c}"{description}, draw={rgb,255:red,92;green,92;blue,214}, from=1-2, to=3-4]
      \arrow["{(\beta *\alpha)_{c'}}"{description}, draw={rgb,255:red,92;green,92;blue,214}, from=5-1, to=7-3]
    \end{tikzcd}
    \begin{aligned}
      &(G'\circ F')(f) \circ (\beta * \alpha)_c\\
      =& (G'\circ F')(f) \circ G'(\alpha_c)\circ\beta_{F(c)}\\
      =& G'(F'(f) \circ \alpha_c)\circ\beta_{F(c)}\\
      =& G'(\alpha_{c'} \circ F)(f) \circ \beta_{F(c)}\\
      =& G'(\alpha_{c'}) \circ (G'\circ F)(f) \circ \beta_{F(c)}\\
      =& G'(\alpha_{c'}) \circ \beta_{F(c')} \circ (G \circ F)(f)\\
      =& (\beta * \alpha)_{c'}\circ (G \circ F)(f)
    \end{aligned}
    \]
  \end{proof}
  \vspace{-\baselineskip}
\end{theorem}

\begin{theorem}[Unitality of Horizontal
  Composition]\label{thm:unitality_horizontal}
  For functors $F, G:\C\to \D$ and a natural transformations
  $\alpha:F\Rightarrow G$, the following holds:
  \[\alpha * \id_{\id_\C} = \id_{\id_\D} * \alpha = \alpha\]

  \begin{proof}
    \[
    \begin{aligned}[t]
      (\alpha * \id_{\id_\C})_C
      &= \alpha_{\id_\C(C)} \circ F\big((\id_{\id_\C})_C\big)\\
      &= \alpha_{C} \circ F(\id_{\id_\C(C)})\\
      &= \alpha_{C} \circ F(\id_{C})\\
      &= \alpha_{C} \circ \id_{F(C)}\\
      &= \alpha_{C}
    \end{aligned}
    \quad
    \begin{aligned}[t]
      (\id_{\id_\D} * \alpha)_C
      &= (\id_{\id_\D})_{G(C)} \circ \id_\D(\alpha_C)\\
      &= \id_{\id_\D(G(C))} \circ \alpha_C\\
      &= \id_{G(C)} \circ \alpha_C\\
      &= \alpha_C
    \end{aligned}
  \]
  \end{proof}
  \vspace{-\baselineskip}
\end{theorem}

\begin{theorem}[Associativity of Horizontal
  Composition]\label{thm:assoc_horizontal}
  For a set-up of categories, functors, and natural transformations:
  % https://q.uiver.app/?q=WzAsNCxbNCwwLCJcXEMiXSxbMiwwLCJcXEIiXSxbMCwwLCJcXEEiXSxbNiwwLCJcXEQiXSxbMSwwLCJHIiwwLHsiY3VydmUiOi00fV0sWzEsMCwiRyciLDIseyJjdXJ2ZSI6NH1dLFsyLDEsIkYiLDAseyJjdXJ2ZSI6LTR9XSxbMiwxLCJGJyIsMix7ImN1cnZlIjo0fV0sWzAsMywiSCIsMCx7ImN1cnZlIjotNH1dLFswLDMsIkgnIiwyLHsiY3VydmUiOjR9XSxbNiw3LCJcXGFscGhhIiwwLHsic2hvcnRlbiI6eyJzb3VyY2UiOjIwLCJ0YXJnZXQiOjIwfX1dLFs0LDUsIlxcYmV0YSIsMCx7InNob3J0ZW4iOnsic291cmNlIjoyMCwidGFyZ2V0IjoyMH19XSxbOCw5LCJcXGdhbW1hIiwwLHsic2hvcnRlbiI6eyJzb3VyY2UiOjIwLCJ0YXJnZXQiOjIwfX1dXQ==&macro_url=https%3A%2F%2Fraw.githubusercontent.com%2Faortega0703%2Fnotes-category-theory%2Fmain%2Fsrc%2Fmacros.tex
  \[\begin{tikzcd}[ampersand replacement=\&]
    \A \&\& \B \&\& \C \&\& \D
    \arrow[""{name=0, anchor=center, inner sep=0}, "G", curve={height=-24pt}, from=1-3, to=1-5]
    \arrow[""{name=1, anchor=center, inner sep=0}, "{G'}"', curve={height=24pt}, from=1-3, to=1-5]
    \arrow[""{name=2, anchor=center, inner sep=0}, "F", curve={height=-24pt}, from=1-1, to=1-3]
    \arrow[""{name=3, anchor=center, inner sep=0}, "{F'}"', curve={height=24pt}, from=1-1, to=1-3]
    \arrow[""{name=4, anchor=center, inner sep=0}, "H", curve={height=-24pt}, from=1-5, to=1-7]
    \arrow[""{name=5, anchor=center, inner sep=0}, "{H'}"', curve={height=24pt}, from=1-5, to=1-7]
    \arrow["\alpha", shorten <=6pt, shorten >=6pt, Rightarrow, from=2, to=3]
    \arrow["\beta", shorten <=6pt, shorten >=6pt, Rightarrow, from=0, to=1]
    \arrow["\gamma", shorten <=6pt, shorten >=6pt, Rightarrow, from=4, to=5]
  \end{tikzcd}\]

  The following holds:
  \[(\gamma * \beta) * \alpha = \gamma * (\beta * \alpha)\]

  \begin{proof}
    % https://q.uiver.app/#q=WzAsOCxbMSwwLCIoSFxcY2lyYyBHXFxjaXJjIEYpKEEpIl0sWzAsMywiKEhcXGNpcmMgR1xcY2lyYyBGJykoQSkiXSxbMywwLCIoSFxcY2lyYyBHJ1xcY2lyYyBGKShBKSJdLFsyLDMsIihIXFxjaXJjIEcnXFxjaXJjIEYnKShBKSJdLFszLDIsIihIJ1xcY2lyYyBHJ1xcY2lyYyBGKShBKSJdLFsxLDIsIihIJ1xcY2lyYyBHXFxjaXJjIEYpKEEpIl0sWzIsNSwiKEgnXFxjaXJjIEcnXFxjaXJjIEYnKShBKSJdLFswLDUsIihIJ1xcY2lyYyBHXFxjaXJjIEYnKShBKSJdLFsyLDQsIlxcZ2FtbWFfeyhHJ1xcY2lyYyBGKShBKX0iLDFdLFswLDUsIlxcZ2FtbWFfeyhHXFxjaXJjIEYpKEEpfSIsMV0sWzMsNiwiXFxnYW1tYV97KEcnXFxjaXJjIEYnKShBKX0iLDFdLFsxLDcsIlxcZ2FtbWFfeyhHXFxjaXJjIEYnKShBKX0iLDFdLFswLDIsIkgoXFxiZXRhX3tGKEEpfSkiLDFdLFs1LDQsIkgnKFxcYmV0YV97RihBKX0pIiwxXSxbMSwzLCJIKFxcYmV0YV97RicoQSl9KSIsMV0sWzcsNiwiSCcoXFxiZXRhX3tGJyhBKX0pIiwxXSxbMiwzLCIoSFxcY2lyYyBHJykoXFxhbHBoYV9BKSIsMV0sWzQsNiwiKEgnXFxjaXJjIEcnKShcXGFscGhhX0EpIiwxXSxbMCwxLCIoSFxcY2lyYyBHKShcXGFscGhhX0EpIiwxXSxbNSw3LCIoSCdcXGNpcmMgRykoXFxhbHBoYV9BKSIsMV0sWzAsMywiSCgoXFxiZXRhKlxcYWxwaGEpX0EpIiwxLHsiY29sb3VyIjpbMjQwLDYwLDYwXX1dLFsxLDYsIihcXGdhbW1hKlxcYmV0YSlfe0YnKEEpfSIsMSx7ImNvbG91ciI6WzI0MCw2MCw2MF19XV0=
    \[\begin{tikzcd}[ampersand replacement=\&,column sep=tiny]
      \& {(H\circ G\circ F)(A)} \&\& {(H\circ G'\circ F)(A)} \\
      \\
      \& {(H'\circ G\circ F)(A)} \&\& {(H'\circ G'\circ F)(A)} \\
      {(H\circ G\circ F')(A)} \&\& {(H\circ G'\circ F')(A)} \\
      \\
      {(H'\circ G\circ F')(A)} \&\& {(H'\circ G'\circ F')(A)}
      \arrow["{\gamma_{(G'\circ F)(A)}}"{description}, from=1-4, to=3-4]
      \arrow["{\gamma_{(G\circ F)(A)}}"{description}, from=1-2, to=3-2]
      \arrow["{\gamma_{(G'\circ F')(A)}}"{description}, from=4-3, to=6-3]
      \arrow["{\gamma_{(G\circ F')(A)}}"{description}, from=4-1, to=6-1]
      \arrow["{H(\beta_{F(A)})}"{description}, from=1-2, to=1-4]
      \arrow["{H'(\beta_{F(A)})}"{description}, from=3-2, to=3-4]
      \arrow["{H(\beta_{F'(A)})}"{description}, from=4-1, to=4-3]
      \arrow["{H'(\beta_{F'(A)})}"{description}, from=6-1, to=6-3]
      \arrow["{(H\circ G')(\alpha_A)}"{description}, from=1-4, to=4-3]
      \arrow["{(H'\circ G')(\alpha_A)}"{description}, from=3-4, to=6-3]
      \arrow["{(H\circ G)(\alpha_A)}"{description}, from=1-2, to=4-1]
      \arrow["{(H'\circ G)(\alpha_A)}"{description}, from=3-2, to=6-1]
      \arrow["{H((\beta*\alpha)_A)}"{description}, draw={rgb,255:red,92;green,92;blue,214}, from=1-2, to=4-3]
      \arrow["{(\gamma*\beta)_{F'(A)}}"{description}, draw={rgb,255:red,92;green,92;blue,214}, from=4-1, to=6-3]
    \end{tikzcd}\]
    \[
      \begin{aligned}
        & ((\gamma * \beta) * \alpha)a\\
        =& (\gamma * \beta)_{F'(a)} \circ (H\circ G)(\alpha_a)\\
        =& \left(\gamma_{(G'\circ F')(a)}\circ H(\beta_{F'(a)})\right)
        \circ (H\circ G)(\alpha_a)\\
        =& \gamma_{(G'\circ F')(a)} \circ
        \left(H(\beta_{F'(a)}) \circ (H\circ G)(\alpha_a)\right)\\
        =& \gamma_{(G'\circ F')(a)} \circ H( (\beta *\alpha)_a)\\
        =& (\gamma * (\beta * \alpha))_a
      \end{aligned}
    \]
  \end{proof}
  \vspace{-\baselineskip}
\end{theorem}

\begin{theorem}
  There is a category with categories as objects and natural transformations as
  morphisms.\

  \begin{proof}
    By Definitions \ref{def:id_nat_transformation},
    \ref{def:nat_transformation_cmp2} and Theorems \ref{thm:assoc_horizontal},
    \ref{thm:unitality_horizontal}
  \end{proof}
\end{theorem}

\begin{definition}[Whiskering]\index{Whiskering}
  For a set-up of categories, functors, and natural transformations:
  % https://q.uiver.app/?q=WzAsMyxbMCwwLCJcXEEiXSxbMSwwLCJcXEIiXSxbMiwwLCJcXEMiXSxbMCwxLCJGIiwwLHsiY3VydmUiOi00fV0sWzAsMSwiRiciLDIseyJjdXJ2ZSI6NH1dLFsxLDIsIkciLDAseyJjdXJ2ZSI6LTR9XSxbMSwyLCJHJyIsMix7ImN1cnZlIjo0fV0sWzMsNCwiXFxhbHBoYSIsMCx7InNob3J0ZW4iOnsic291cmNlIjoyMCwidGFyZ2V0IjoyMH19XSxbNSw2LCJcXGJldGEiLDAseyJzaG9ydGVuIjp7InNvdXJjZSI6MjAsInRhcmdldCI6MjB9fV1d&macro_url=https%3A%2F%2Fraw.githubusercontent.com%2Faortega0703%2Fnotes-category-theory%2Fmain%2Fsrc%2Fmacros.tex
  \[\begin{tikzcd}[ampersand replacement=\&]
    \A \& \B \& \C
    \arrow[""{name=0, anchor=center, inner sep=0}, "F", curve={height=-24pt}, from=1-1, to=1-2]
    \arrow[""{name=1, anchor=center, inner sep=0}, "{F'}"', curve={height=24pt}, from=1-1, to=1-2]
    \arrow[""{name=2, anchor=center, inner sep=0}, "G", curve={height=-24pt}, from=1-2, to=1-3]
    \arrow[""{name=3, anchor=center, inner sep=0}, "{G'}"', curve={height=24pt}, from=1-2, to=1-3]
    \arrow["\alpha", shorten <=6pt, shorten >=6pt, Rightarrow, from=0, to=1]
    \arrow["\beta", shorten <=6pt, shorten >=6pt, Rightarrow, from=2, to=3]
  \end{tikzcd}\]

  Whiskering between functors and natural transformations is defined as:
  \[
    \begin{aligned}
      (\beta \circ F)_a &\coloneqq \beta_{F(a)}
    \end{aligned}
    \quad
    \begin{aligned}
      (G \circ \alpha)_a &\coloneqq G(\alpha_a)
    \end{aligned}
  \]
\end{definition}

\begin{remark}
  The definition of whiskering is motivated by considering the horizontal
  compositions with functor identities:
  %% https://q.uiver.app/#q=WzAsNCxbMCwwLCIoR1xcY2lyYyBGKShhKSJdLFsxLDEsIihHJ1xcY2lyYyBGKShhKSJdLFsxLDAsIihHJ1xcY2lyYyBGKShhKSJdLFswLDEsIihHXFxjaXJjIEYpKGEpIl0sWzAsMiwiXFxiZXRhX3tGKGEpfSJdLFswLDMsIkcoXFxpZF97RihhKX0pIiwyXSxbMCwxLCJcXGJldGEqXFxpZF9GIiwxXSxbMywxLCJcXGJldGFfe0YoYSl9IiwyXSxbMiwxLCJHJyhcXGlkX3tGKGEpfSkiXV0=&macro_url=https%3A%2F%2Fgist.githubusercontent.com%2Faortega0703%2Fa1fd97cb097b8142e63a6fbf0cdb0f76%2Fraw%2Fe6ec84fda0ef3d3ac45c61c03814b7a3a1c30dff%2Fmacros.tex
  \[\begin{tikzcd}[ampersand replacement=\&]
    {(G\circ F)(a)} \& {(G'\circ F)(a)} \\
    {(G\circ F)(a)} \& {(G'\circ F)(a)}
    \arrow["{\beta_{F(a)}}", from=1-1, to=1-2]
    \arrow["{G(\id_{F(a)})}"', from=1-1, to=2-1]
    \arrow["{\beta*\id_F}"{description}, from=1-1, to=2-2]
    \arrow["{\beta_{F(a)}}"', from=2-1, to=2-2]
    \arrow["{G'(\id_{F(a)})}", from=1-2, to=2-2]
  \end{tikzcd}
  \quad
  % https://q.uiver.app/#q=WzAsNCxbMCwwLCIoR1xcY2lyYyBGKShhKSJdLFsxLDEsIihHXFxjaXJjIEYnKShhKSJdLFsxLDAsIihHXFxjaXJjIEYpKGEpIl0sWzAsMSwiKEdcXGNpcmMgRicpKGEpIl0sWzAsMiwiKFxcaWRfRylfe0YoYSl9Il0sWzIsMSwiRyhcXGFscGhhX2EpIl0sWzAsMywiRyhcXGFscGhhX2EpIiwyXSxbMywxLCIoXFxpZF9HKV97RihhKX0iLDJdLFswLDEsIlxcaWRfRyAqIFxcYWxwaGEiLDFdXQ==&macro_url=https%3A%2F%2Fgist.githubusercontent.com%2Faortega0703%2Fa1fd97cb097b8142e63a6fbf0cdb0f76%2Fraw%2Fe6ec84fda0ef3d3ac45c61c03814b7a3a1c30dff%2Fmacros.tex
  \begin{tikzcd}[ampersand replacement=\&]
    {(G\circ F)(a)} \& {(G\circ F)(a)} \\
    {(G\circ F')(a)} \& {(G\circ F')(a)}
    \arrow["{(\id_G)_{F(a)}}", from=1-1, to=1-2]
    \arrow["{G(\alpha_a)}", from=1-2, to=2-2]
    \arrow["{G(\alpha_a)}"', from=1-1, to=2-1]
    \arrow["{(\id_G)_{F(a)}}"', from=2-1, to=2-2]
    \arrow["{\id_G * \alpha}"{description}, from=1-1, to=2-2]
  \end{tikzcd}\]
\end{remark}

\begin{theorem}[Interchange Law]
  For a set-up of categories, functors, and natural transformations:
  % https://q.uiver.app/?q=WzAsMyxbNCwwLCJcXEMiXSxbMiwwLCJcXEIiXSxbMCwwLCJcXEEiXSxbMSwwLCJHXzEiLDAseyJjdXJ2ZSI6LTR9XSxbMSwwLCJHXzMiLDIseyJjdXJ2ZSI6NH1dLFsyLDEsIkZfMSIsMCx7ImN1cnZlIjotNH1dLFsyLDEsIkZfMiIsMV0sWzIsMSwiRl8zIiwyLHsiY3VydmUiOjR9XSxbMSwwLCJHXzIiLDFdLFs1LDYsIlxcYWxwaGFfMSIsMCx7InNob3J0ZW4iOnsic291cmNlIjoyMCwidGFyZ2V0IjoyMH19XSxbNiw3LCJcXGFscGhhXzIiLDAseyJzaG9ydGVuIjp7InNvdXJjZSI6MjAsInRhcmdldCI6MjB9fV0sWzMsOCwiXFxiZXRhXzEiLDAseyJzaG9ydGVuIjp7InNvdXJjZSI6MjAsInRhcmdldCI6MjB9fV0sWzgsNCwiXFxiZXRhXzIiLDAseyJzaG9ydGVuIjp7InNvdXJjZSI6MjAsInRhcmdldCI6MjB9fV1d&macro_url=https%3A%2F%2Fraw.githubusercontent.com%2Faortega0703%2Fnotes-category-theory%2Fmain%2Fsrc%2Fmacros.tex
  \[\begin{tikzcd}[ampersand replacement=\&]
    \A \&\& \B \&\& \C
    \arrow[""{name=0, anchor=center, inner sep=0}, "{G_1}", curve={height=-24pt}, from=1-3, to=1-5]
    \arrow[""{name=1, anchor=center, inner sep=0}, "{G_3}"', curve={height=24pt}, from=1-3, to=1-5]
    \arrow[""{name=2, anchor=center, inner sep=0}, "{F_1}", curve={height=-24pt}, from=1-1, to=1-3]
    \arrow[""{name=3, anchor=center, inner sep=0}, "{F_2}"{description}, from=1-1, to=1-3]
    \arrow[""{name=4, anchor=center, inner sep=0}, "{F_3}"', curve={height=24pt}, from=1-1, to=1-3]
    \arrow[""{name=5, anchor=center, inner sep=0}, "{G_2}"{description}, from=1-3, to=1-5]
    \arrow["{\alpha_1}", shorten <=3pt, shorten >=3pt, Rightarrow, from=2, to=3]
    \arrow["{\alpha_2}", shorten <=3pt, shorten >=3pt, Rightarrow, from=3, to=4]
    \arrow["{\beta_1}", shorten <=3pt, shorten >=3pt, Rightarrow, from=0, to=5]
    \arrow["{\beta_2}", shorten <=3pt, shorten >=3pt, Rightarrow, from=5, to=1]
  \end{tikzcd}\]

  The following holds:
  \[(\beta_2\circ\beta_1)*(\alpha_2\circ\alpha_1) = (\beta_2*\alpha_2) \circ
  (\alpha_2*\alpha_2)\]

  \begin{proof}
    Consider the following diagram in the exponential category $\A^\C$:

    % https://q.uiver.app/?q=WzAsOSxbMCwwLCJHXzFcXGNpcmMgRl8xIl0sWzIsMiwiR18yXFxjaXJjIEZfMiJdLFsyLDAsIkdfMlxcY2lyYyBGXzEiXSxbMCwyLCJHXzEgXFxjaXJjIEZfMiJdLFs0LDQsIkdfMyBcXGNpcmMgRl8zIl0sWzAsNCwiR18xIFxcY2lyYyBGXzMiXSxbMiw0LCJHXzJcXGNpcmMgRl8zIl0sWzQsMiwiR18zIFxcY2lyYyBGXzIiXSxbNCwwLCJHXzNcXGNpcmMgRl8xIl0sWzAsMSwiXFxiZXRhXzEqXFxhbHBoYV8xIiwxXSxbMCwyLCJcXGJldGFfMVxcY2lyYyBGXzEiLDFdLFswLDMsIkdfMVxcY2lyY1xcYWxwaGFfMSIsMV0sWzMsMSwiXFxiZXRhXzFcXGNpcmMgRl8yIiwxXSxbMiwxLCJHXzJcXGNpcmMgXFxhbHBoYV8xIiwxXSxbMSw0LCJcXGJldGFfMiAqIFxcYWxwaGFfMiIsMV0sWzMsNSwiR18xXFxjaXJjXFxhbHBoYV8yIiwxXSxbNSw2LCJcXGJldGFfMVxcY2lyYyBGXzMiLDFdLFszLDYsIlxcYmV0YV8xKlxcYWxwaGFfMiIsMV0sWzEsNiwiR18yXFxjaXJjXFxhbHBoYV8yIiwxXSxbNiw0LCJcXGJldGFfMlxcY2lyYyBGXzMiLDFdLFsxLDcsIlxcYmV0YV8yXFxjaXJjIEZfMiIsMV0sWzcsNCwiR18zXFxjaXJjIFxcYWxwaGFfMiIsMV0sWzIsOCwiXFxiZXRhXzJcXGNpcmMgRjEiLDFdLFs4LDcsIkdfM1xcY2lyY1xcYWxwaGFfMSIsMV0sWzIsNywiXFxiZXRhXzIqXFxhbHBoYV8xIiwxXV0=&macro_url=https%3A%2F%2Fgist.githubusercontent.com%2Faortega0703%2Fa1fd97cb097b8142e63a6fbf0cdb0f76%2Fraw%2Fe6ec84fda0ef3d3ac45c61c03814b7a3a1c30dff%2Fmacros.tex
    \[\begin{tikzcd}[ampersand replacement=\&]
      {G_1\circ F_1} \&\& {G_2\circ F_1} \&\& {G_3\circ F_1} \\
      \\
      {G_1 \circ F_2} \&\& {G_2\circ F_2} \&\& {G_3 \circ F_2} \\
      \\
      {G_1 \circ F_3} \&\& {G_2\circ F_3} \&\& {G_3 \circ F_3}
      \arrow["{\beta_1*\alpha_1}"{description}, from=1-1, to=3-3]
      \arrow["{\beta_1\circ F_1}"{description}, from=1-1, to=1-3]
      \arrow["{G_1\circ\alpha_1}"{description}, from=1-1, to=3-1]
      \arrow["{\beta_1\circ F_2}"{description}, from=3-1, to=3-3]
      \arrow["{G_2\circ \alpha_1}"{description}, from=1-3, to=3-3]
      \arrow["{\beta_2 * \alpha_2}"{description}, from=3-3, to=5-5]
      \arrow["{G_1\circ\alpha_2}"{description}, from=3-1, to=5-1]
      \arrow["{\beta_1\circ F_3}"{description}, from=5-1, to=5-3]
      \arrow["{\beta_1*\alpha_2}"{description}, from=3-1, to=5-3]
      \arrow["{G_2\circ\alpha_2}"{description}, from=3-3, to=5-3]
      \arrow["{\beta_2\circ F_3}"{description}, from=5-3, to=5-5]
      \arrow["{\beta_2\circ F_2}"{description}, from=3-3, to=3-5]
      \arrow["{G_3\circ \alpha_2}"{description}, from=3-5, to=5-5]
      \arrow["{\beta_2\circ F1}"{description}, from=1-3, to=1-5]
      \arrow["{G_3\circ\alpha_1}"{description}, from=1-5, to=3-5]
      \arrow["{\beta_2*\alpha_1}"{description}, from=1-3, to=3-5]
    \end{tikzcd}\]

    \[
      \begin{aligned}
        (\beta_2 \circ \beta_1) * (\alpha_2 \circ \alpha_1)
        &= (G_3\circ \alpha_2) \circ (G_3\circ \alpha_1)
          \circ (beta_2 \circ F1) \circ (\beta_1 \circ F1)\\
        &= (G_3\circ \alpha_2) \circ (\beta_2\circ F_2)
          \circ (G_2\circ \alpha_1) \circ (\beta_1\circ F_1)\\
        &= (\beta_2 * \alpha_2) \circ (\beta_1 * \alpha_1)
      \end{aligned}
    \]
  \end{proof}
  \vspace{-1.5\baselineskip}
\end{theorem}