\subsection{Identity}

\begin{definition}[Identity Natural Transformation\index{Identity Natural Transformation}]
  For a functor $F:\C\to \D$, there exists a natural transformation $\id_F:
  F\Rightarrow F$ which consists
  of~\parencite[p.~30]{leinster:basic_category_theory}:

  \begin{itemize}
    \item $c$-Components:
      \[(\forall c\in \C_0)
        \big((\id_F)_c = \id_{F(c)}\big)\]
    \item Naturality Condition:
      % https://q.uiver.app/?q=WzAsNCxbMCwwLCJGKGMpIl0sWzEsMCwiRihjJykiXSxbMCwxLCJGKGMpIl0sWzEsMSwiRihjJykiXSxbMCwxLCJGKGYpIl0sWzAsMiwiXFxtYXRocm17aWR9X3tGKGMpfSIsMl0sWzIsMywiRihmKSIsMl0sWzEsMywiXFxtYXRocm17aWR9X3tGKGMnKX0iXV0=
      \[\begin{tikzcd}
        {F(c)} & {F(c')} \\
        {F(c)} & {F(c')}
        \arrow["{F(f)}", from=1-1, to=1-2]
        \arrow["{\mathrm{id}_{F(c)}}"', from=1-1, to=2-1]
        \arrow["{F(f)}"', from=2-1, to=2-2]
        \arrow["{\mathrm{id}_{F(c')}}", from=1-2, to=2-2]
      \end{tikzcd}\]
  \end{itemize}
\end{definition}

\begin{theorem}[Naturality of Identity Natural Transformation]
  The naturality condition of the identity natural transformation holds.

  \begin{proof}
    By unitality it follows that $F(f) \circ \id_{F(c)} = \id_{F(c')} \circ
    F(f)$.
  \end{proof}
\end{theorem}